CoqOfRust/core/simulations/clone.v
@@ -16,11 +16,12 @@ Import Run.
 Module Clone.
   Record RunImpl `{State.Trait} (Self : Set) `{ToTy Self} `{ToValue Self} : Set := {
     clone : {clone @
-      IsTraitMethod "core::clone::Clone" (Φ Self) [] "clone" clone *
+      IsTraitMethod.t "core::clone::Clone" (Φ Self) [] "clone" clone *
       forall (state : State) (pointer : Pointer.t Value.t),
         HasRead.t state pointer φ ->
-        {{ _, _, state |
-          clone [] [ Value.Pointer pointer ] ⇓ (fun v => inl (φ v))
+        {{ _, state |
+          clone [] [ Value.Pointer pointer ] ⇓
+          fun (v : Self) => inl (φ v)
         | fun state' => state' = state }}
     };
     (* TODO: add [clone_from] *)
